code/ecdsap256/Hacl.Impl.P256.Bignum.fst
@@ -293,7 +293,7 @@ let mul1_il f u result =
   let temp0 = index temp (size 0) in
     lemma_low_level0 (uint_v(Seq.index (as_seq h1 o0) 0)) (uint_v (Seq.index (as_seq h2 o1) 0)) (uint_v (Seq.index (as_seq h3 o2) 0)) (uint_v (Seq.index (as_seq h4 o3) 0)) (uint_v f0) (uint_v f1) (uint_v f2) (uint_v f3) (uint_v u) (uint_v (Seq.index (as_seq h2 temp) 0)) (uint_v c1) (uint_v c2) (uint_v c3) (uint_v (Seq.index (as_seq h3 temp) 0)) (uint_v temp0);
 
-  Spec.P256.Lemmas.mul_lemma_4 (as_nat_il h0 f) (uint_v u) (pow2 256 - 1) (pow2 64 - 1);
+  Hacl.Spec.P256.Lemmas.mul_lemma_4 (as_nat_il h0 f) (uint_v u) (pow2 256 - 1) (pow2 64 - 1);
   assert_norm((pow2 256 - 1) * (pow2 64 - 1) == pow2 320 - pow2 256 - pow2 64 + 1);
   assert_norm((pow2 320 - pow2 256) / pow2 256 == pow2 64 - 1);
 
