code/ecdsap256/Hacl.Impl.P256.Constants.fst
@@ -1,0 +1,167 @@
+module Hacl.Impl.P256.Constants
+
+open FStar.Mul
+open FStar.HyperStack.All
+open FStar.HyperStack
+module ST = FStar.HyperStack.ST
+
+open Lib.IntTypes
+open Lib.Buffer
+
+module S = Spec.P256
+module LSeq = Lib.Sequence
+module BSeq = Lib.ByteSequence
+
+open Hacl.Spec.P256.Felem
+
+#set-options "--z3rlimit 50"
+
+inline_for_extraction noextract
+let p256_prime_list : x:list uint64{List.Tot.length x == 4 /\
+  (
+    let l0 = uint_v (List.Tot.index x 0) in
+    let l1 = uint_v (List.Tot.index x 1) in
+    let l2 = uint_v (List.Tot.index x 2) in
+    let l3 = uint_v (List.Tot.index x 3) in
+    l0 + l1 * pow2 64 + l2 * pow2 128 + l3 * pow2 192 == S.prime256)
+  } =
+  [@inline_let]
+  let x =
+    [ u64 0xffffffffffffffff; u64 0xffffffff; u64 0; u64 0xffffffff00000001] in
+    assert_norm (0xffffffffffffffff + 0xffffffff * pow2 64 + 0xffffffff00000001 * pow2 192 == S.prime256);
+  x
+
+
+inline_for_extraction noextract
+let p256_order_prime_list : x:list uint64{List.Tot.length x == 4 /\
+  (
+    let l0 = uint_v (List.Tot.index x 0) in
+    let l1 = uint_v (List.Tot.index x 1) in
+    let l2 = uint_v (List.Tot.index x 2) in
+    let l3 = uint_v (List.Tot.index x 3) in
+    l0 + l1 * pow2 64 + l2 * pow2 128 + l3 * pow2 192 == S.prime_p256_order)
+  } =
+  [@inline_let]
+  let x =
+    [ u64 17562291160714782033; u64 13611842547513532036; u64 18446744073709551615; u64 18446744069414584320 ] in
+    assert_norm (17562291160714782033 + 13611842547513532036 * pow2 64 + 18446744073709551615* pow2 128 + 18446744069414584320 * pow2 192 == S.prime_p256_order);
+  x
+
+
+let prime256_buffer: x: glbuffer uint64 4ul {
+  witnessed #uint64 #(size 4) x (LSeq.of_list p256_prime_list) /\
+  recallable x /\
+  felem_seq_as_nat (LSeq.of_list (p256_prime_list)) == S.prime256} =
+
+  assert_norm (felem_seq_as_nat (LSeq.of_list (p256_prime_list)) == S.prime256);
+  createL_global p256_prime_list
+
+
+let prime256order_buffer: x: glbuffer uint64 (size 4) {
+  witnessed #uint64 #(size 4) x (LSeq.of_list p256_order_prime_list) /\
+  recallable x /\
+  felem_seq_as_nat (LSeq.of_list (p256_order_prime_list)) == S.prime_p256_order} =
+  createL_global p256_order_prime_list
+
+
+//--------------------------------
+// TODO: rm
+
+#push-options "--ifuel 1"
+val nat_from_intlist_le: #t:inttype{unsigned t} -> #l:secrecy_level -> list (uint_t t l) -> nat
+let rec nat_from_intlist_le #t #l = function
+  | [] -> 0
+  | hd :: tl -> v hd + pow2 (bits t) * nat_from_intlist_le tl
+
+val nat_from_intlist_be: #t:inttype{unsigned t} -> #l:secrecy_level -> list (uint_t t l) -> nat
+let rec nat_from_intlist_be #t #l = function
+  | [] -> 0
+  | hd :: tl -> pow2 (FStar.List.Tot.Base.length tl * bits t) * v hd + nat_from_intlist_be tl
+#pop-options
+
+
+#push-options "--fuel 1"
+val index_seq_of_list_cons: #a:Type -> x:a -> l:list a -> i:nat{i < List.Tot.length l} -> Lemma
+  (Seq.index (Seq.seq_of_list (x::l)) (i+1) == Seq.index (Seq.seq_of_list l) i)
+
+let index_seq_of_list_cons #a x l i =
+  assert (Seq.index (Seq.seq_of_list (x::l)) (i+1) == List.Tot.index (x::l) (i+1))
+
+val nat_from_intlist_seq_le: #t:inttype{unsigned t} -> #l:secrecy_level
+  -> len:size_nat -> b:list (uint_t t l){List.Tot.length b = len}
+  -> Lemma (nat_from_intlist_le b == BSeq.nat_from_intseq_le (LSeq.of_list b))
+
+let rec nat_from_intlist_seq_le #t #l len b =
+  match b with
+  | [] -> ()
+  | hd :: tl ->
+    begin
+    let s = LSeq.of_list b in
+    Classical.forall_intro (index_seq_of_list_cons hd tl);
+    assert (LSeq.equal (LSeq.of_list tl) (LSeq.slice s 1 len));
+    assert (LSeq.index s 0 == List.Tot.index b 0);
+    BSeq.nat_from_intseq_le_lemma0 (LSeq.slice s 0 1);
+    BSeq.nat_from_intseq_le_slice_lemma s 1;
+    nat_from_intlist_seq_le (len - 1) tl
+    end
+
+
+val nat_from_intlist_seq_be: #t: inttype {unsigned t} -> #l: secrecy_level
+  -> len: size_nat -> b: list (uint_t t l) {FStar.List.Tot.Base.length b = len}
+  -> Lemma (nat_from_intlist_be b == BSeq.nat_from_intseq_be (LSeq.of_list b))
+
+let rec nat_from_intlist_seq_be #t #l len b =
+  match b with
+  | [] -> ()
+  | hd :: tl ->
+    begin
+      let s = LSeq.of_list b in
+      Classical.forall_intro (index_seq_of_list_cons hd tl);
+      assert (LSeq.equal (LSeq.of_list tl) (LSeq.slice s 1 len));
+      assert (LSeq.index s 0 == List.Tot.index b 0);
+      nat_from_intlist_seq_be (len - 1) tl;
+      BSeq.nat_from_intseq_be_lemma0 (LSeq.slice s 0 1);
+      BSeq.nat_from_intseq_be_slice_lemma s 1
+      end
+#pop-options
+
+
+unfold let prime_p256_order_inverse_list: list uint8 =
+ [
+   u8 79;  u8 37;  u8 99;  u8 252; u8 194; u8 202; u8 185; u8 243;
+   u8 132; u8 158; u8 23;  u8 167; u8 173; u8 250; u8 230; u8 188;
+   u8 255; u8 255; u8 255; u8 255; u8 255; u8 255; u8 255; u8 255;
+   u8 0;   u8 0;   u8 0;   u8 0;   u8 255; u8 255; u8 255; u8 255
+ ]
+
+
+let prime_p256_order_inverse_seq: s:LSeq.lseq uint8 32{BSeq.nat_from_intseq_le s == S.prime_p256_order - 2} =
+  assert_norm (List.Tot.length prime_p256_order_inverse_list == 32);
+  nat_from_intlist_seq_le 32 prime_p256_order_inverse_list;
+  assert_norm (nat_from_intlist_le prime_p256_order_inverse_list == S.prime_p256_order - 2);
+  LSeq.of_list prime_p256_order_inverse_list
+
+
+unfold let prime_p256_order_list: list uint8 =
+ [
+  u8 255; u8 255; u8 255; u8 255; u8 0;  u8 0;   u8 0;   u8 0;
+  u8 255; u8 255; u8 255; u8 255; u8 255; u8 255; u8 255; u8 255;
+  u8 188; u8 230; u8 250; u8 173; u8 167; u8 23; u8 158; u8 132;
+  u8 243; u8 185; u8 202; u8 194; u8 252; u8 99; u8 37; u8 81
+ ]
+
+
+let prime_p256_order_seq: s:LSeq.lseq uint8 32{BSeq.nat_from_intseq_be s == S.prime_p256_order} =
+  assert_norm (List.Tot.length prime_p256_order_list == 32);
+  nat_from_intlist_seq_be 32 prime_p256_order_list;
+  assert_norm (nat_from_intlist_be prime_p256_order_list == S.prime_p256_order);
+  LSeq.of_list prime_p256_order_list
+
+
+// NOTE: used in Hacl.Impl.ECDSA.MM.Exponent.fst
+let order_inverse_buffer: x: glbuffer uint8 32ul {witnessed x prime_p256_order_inverse_seq /\ recallable x} =
+  createL_global prime_p256_order_inverse_list
+
+
+let order_buffer: x: glbuffer uint8 32ul {witnessed x prime_p256_order_seq /\ recallable x} =
+  createL_global prime_p256_order_list
