code/ecdsap256/Hacl.Impl.P256.Field.fst
@@ -11,12 +11,14 @@ open Lib.IntTypes
 open Lib.Buffer
 open Lib.IntTypes.Intrinsics
 
-open Spec.P256.Constants
+open Spec.P256
+open Hacl.Spec.P256.Lemmas
 open Hacl.Spec.P256.MontgomeryMultiplication
 
 open Hacl.Spec.P256.Felem
 open Hacl.Impl.P256.Bignum
 open Hacl.Impl.P256.Math
+open Hacl.Impl.P256.Constants
 
 #set-options "--z3rlimit 50 --fuel 0 --ifuel 0"
 
