code/ecdsap256/Hacl.Impl.P256.Field.fsti
@@ -8,23 +8,11 @@ module ST = FStar.HyperStack.ST
 open Lib.IntTypes
 open Lib.Buffer
 
-open Spec.P256.Constants
-open Spec.P256.Lemmas
+open Spec.P256
 open Hacl.Spec.P256.MontgomeryMultiplication
-
 open Hacl.Spec.P256.Felem
 
 #set-options "--z3rlimit 50"
-
-// TODO: fix and mv
-let prime256_buffer: x: glbuffer uint64 4ul {
-  witnessed #uint64 #(size 4) x (Lib.Sequence.of_list p256_prime_list) /\
-  recallable x /\
-  felem_seq_as_nat (Lib.Sequence.of_list (p256_prime_list)) == prime256} =
-
-  assert_norm (felem_seq_as_nat (Lib.Sequence.of_list (p256_prime_list)) == prime256);
-  createL_global p256_prime_list
-
 
 val fmod_short: x:felem -> res:felem -> Stack unit
   (requires fun h ->
