code/ecdsap256/Hacl.Impl.P256.Point.fsti
@@ -8,10 +8,9 @@ open Lib.IntTypes
 open Lib.Buffer
 
 open Spec.P256
-open Spec.P256.Constants
-open Hacl.Spec.P256.MontgomeryMultiplication
 open Spec.ECDSA
 
+open Hacl.Spec.P256.MontgomeryMultiplication
 open Hacl.Spec.P256.Felem
 
 module LSeq = Lib.Sequence
