code/ecdsap256/Hacl.Impl.P256.Qinv.fst
@@ -11,7 +11,8 @@ open FStar.Math.Lemmas
 open Hacl.Impl.P256.Math
 
 open Hacl.Impl.P256.Bignum
-open Spec.P256.Lemmas
+open Hacl.Impl.P256.Constants
+open Hacl.Spec.P256.Lemmas
 open FStar.Tactics
 open FStar.Tactics.Canon
 
