code/ecdsap256/Hacl.Impl.P256.Scalar.fst
@@ -13,10 +13,11 @@ open Lib.IntTypes
 open Lib.Buffer
 open Lib.IntTypes.Intrinsics
 
-open Spec.P256.Lemmas
-open Spec.P256.Constants
+open Hacl.Spec.P256.Lemmas
+open Spec.P256
 
 open Hacl.Impl.P256.Bignum
+open Hacl.Impl.P256.Constants
 
 #reset-options "--z3rlimit 200 --fuel 0 --ifuel 0"
 
