code/ecdsap256/Hacl.Spec.P256.MontgomeryMultiplication.fst
@@ -7,11 +7,11 @@ open FStar.Mul
 open Lib.IntTypes
 open Lib.ByteSequence
 
-open Spec.P256.Lemmas
-open Spec.P256.Constants
 open Spec.P256
+open Hacl.Spec.P256.Lemmas
 
 #set-options "--z3rlimit 40 --fuel 0 --ifuel 0"
+
 
 let prime = prime256
 
