code/ecdsap256/Hacl.Spec.P256.MontgomeryMultiplication.fsti
@@ -7,11 +7,9 @@ open FStar.Mul
 open Lib.IntTypes
 open Lib.Sequence
 
-open Spec.P256.Lemmas
-open Spec.P256.Constants
+open Spec.P256
 
 #set-options "--z3rlimit 40 --fuel 0 --ifuel 0"
-
 
 // used in Spec.P256.Montgomerymultiplication.PointAdd
 val fromDomain_: a: int -> Tot (a: nat {a < prime256})
