code/tests/Hacl.Test.ECDSA.fst
@@ -207,12 +207,12 @@ val check_bound: b:Lib.Buffer.lbuffer uint8 32ul -> Stack bool
       (
 	(Lib.ByteSequence.nat_from_bytes_be (Lib.Buffer.as_seq h0 b) > 0) &&
 	(Lib.ByteSequence.nat_from_bytes_be (Lib.Buffer.as_seq h0 b) <
-          Spec.P256.Constants.prime_p256_order)))
+          Spec.P256.prime_p256_order)))
 
 let check_bound b =
   let open FStar.Mul in
   let open Lib.ByteSequence in
-  let open Spec.P256.Constants in
+  let open Spec.P256 in
   [@inline_let]
   let q1 = normalize_term (prime_p256_order % pow2 64) in 
   [@inline_let]
